compiler/src/compiler/regs_initialized.v
@@ -1,0 +1,45 @@
+Require Import Coq.ZArith.ZArith.
+Require Import coqutil.Map.Interface coqutil.Map.Properties.
+Require Import coqutil.Tactics.Tactics.
+Local Open Scope Z_scope.
+
+Section WithParameters.
+  Context {width: Z} {T: Type} {locals: map.map Z T} {locals_ok: map.ok locals}.
+
+  Definition regs_initialized(regs: locals): Prop :=
+    forall r : Z, 0 < r < 32 -> exists v : T, map.get regs r = Some v.
+
+  Lemma regs_initialized_put: forall l x v,
+      regs_initialized l ->
+      regs_initialized (map.put l x v).
+  Proof.
+    unfold regs_initialized in *.
+    intros.
+    rewrite map.get_put_dec.
+    destruct_one_match; eauto.
+  Qed.
+
+  Lemma preserve_regs_initialized_after_put: forall regs var val,
+      regs_initialized regs ->
+      regs_initialized (map.put regs var val).
+  Proof.
+    unfold regs_initialized. intros. specialize (H _ H0).
+    rewrite map.get_put_dec. destruct_one_match; subst; eauto.
+  Qed.
+
+  Lemma preserve_regs_initialized_after_putmany_of_list_zip: forall vars vals (regs regs': locals),
+      regs_initialized regs ->
+      map.putmany_of_list_zip vars vals regs = Some regs' ->
+      regs_initialized regs'.
+  Proof.
+    induction vars; intros.
+    - simpl in H0. destruct vals; try discriminate.
+      replace regs' with regs in * by congruence. assumption.
+    - simpl in H0.
+      destruct vals; try discriminate.
+      eapply IHvars. 2: eassumption.
+      eapply preserve_regs_initialized_after_put.
+      eassumption.
+  Qed.
+
+End WithParameters.
